# baseURI: http://geophy.io/ontologies/glossary
# imports: https://www.dublincore.org/specifications/dublin-core/dcmi-terms/dublin_core_terms.ttl
# prefix: glossary

@prefix glossary: <http://geophy.io/ontologies/glossary#> .
@prefix owl: <http://www.w3.org/2002/07/owl#> .
@prefix rdf: <http://www.w3.org/1999/02/22-rdf-syntax-ns#> .
@prefix rdfs: <http://www.w3.org/2000/01/rdf-schema#> .
@prefix xsd: <http://www.w3.org/2001/XMLSchema#> .

<http://geophy.io/ontologies/glossary>
  a owl:Ontology ;
  owl:imports <https://www.dublincore.org/specifications/dublin-core/dcmi-terms/dublin_core_terms.ttl> ;
  owl:versionInfo "Created with TopBraid Composer" ;
.
glossary:Term
  a owl:Class ;
  rdfs:comment "glossary:Term is used to capture the formal definition and explanation related to a term. These terms are often classfiied using a specific category and subcategory." ;
  rdfs:label "Term" ;
  rdfs:subClassOf owl:Thing ;
.
glossary:TermCategory
  a owl:Class ;
  rdfs:comment "glossary:termCategory is a controlled vocabulary that lists the expected catogories for the defined terms." ;
  rdfs:label "Term" ;
  rdfs:subClassOf owl:Thing ;
.
glossary:TermSubcategory
  a owl:Class ;
  rdfs:comment "glossary:termSubcategory is a controlled vocabulary that lists the expected sub-catogories for the defined terms." ;
  rdfs:label "Term" ;
  rdfs:subClassOf owl:Thing ;
.
glossary:hasCategory
  a owl:ObjectProperty ;
  rdfs:comment "The object property that connects a defined term with its category." ;
  rdfs:domain glossary:Term ;
  rdfs:label "hasCategory" ;
  rdfs:range glossary:TermCategory ;
.
glossary:hasSubcategory
  a owl:ObjectProperty ;
  rdfs:comment "The object property that connects a defined term with its subcategory." ;
  rdfs:domain glossary:Term ;
  rdfs:label "hasSubcategory" ;
  rdfs:range glossary:TermSubcategory ;
.
glossary:rationale
  a owl:DatatypeProperty ;
  rdfs:comment "glossary:rationale is a data property that captures the reason of the existence of the defined term." ;
  rdfs:domain glossary:Term ;
  rdfs:label "rationale" ;
  rdfs:range xsd:string ;
.
<http://purl.org/dc/terms/description>
  rdfs:domain glossary:Term ;
.
