# baseURI: http://geophy.io/ontologies/ml
# imports: http://geophy.io/ontologies/fcat
# imports: http://purl.org/dc/elements/1.1/
# imports: http://purl.org/dc/terms/
# prefix: ml

@prefix : <http://geophy.io/ontologies/ml#> .
@prefix ml: <http://geophy.io/ontologies/ml#> .
@prefix owl: <http://www.w3.org/2002/07/owl#> .
@prefix rdf: <http://www.w3.org/1999/02/22-rdf-syntax-ns#> .
@prefix rdfs: <http://www.w3.org/2000/01/rdf-schema#> .
@prefix xsd: <http://www.w3.org/2001/XMLSchema#> .

<http://geophy.io/ontologies/ml>
  a owl:Ontology ;
  owl:imports <http://geophy.io/ontologies/fcat> ;
  owl:imports <http://purl.org/dc/elements/1.1/> ;
  owl:imports <http://purl.org/dc/terms/> ;
  owl:versionInfo "Created with TopBraid Composer" ;
.
ml:Model
  a owl:Class ;
  rdfs:comment "ml:model represents a machine learning model instance. It is used to captures the metadata around an ML model." ;
  rdfs:label "Model" ;
.
ml:hasInputFeature
  a owl:ObjectProperty ;
  rdfs:comment "ml:hasFeature is superclass of the different types of features used in an ML model." ;
  rdfs:domain ml:Model ;
  rdfs:label "hasInputFeature" ;
  rdfs:range <http://geophy.io/ontologies/fcat#Feature> ;
  rdfs:subPropertyOf owl:topObjectProperty ;
.
ml:hasModelFeature
  a owl:ObjectProperty ;
  rdfs:comment "ml:hasModelFeature is an object property that connects a machine learning model instance with a feature that is used as a model feature in the ML model." ;
  rdfs:domain ml:Model ;
  rdfs:label "hasModelFeature" ;
  rdfs:range <http://geophy.io/ontologies/fcat#Feature> ;
  rdfs:subPropertyOf ml:hasInputFeature ;
.
ml:hasNonModelFeature
  a owl:ObjectProperty ;
  rdfs:comment "ml:hasNonModelFeature is an object property that connects a machine learning model instance with a feature that is used only as an imputation feature in the ML model." ;
  rdfs:domain ml:Model ;
  rdfs:label "hasNonModelFeature" ;
  rdfs:range <http://geophy.io/ontologies/fcat#Feature> ;
  rdfs:subPropertyOf ml:hasInputFeature ;
.
<http://purl.org/dc/terms/description>
  rdfs:domain ml:Model ;
.
<http://purl.org/dc/terms/hasVersion>
  rdfs:domain ml:Model ;
.
